\section*{Aufgabe 1}
\paragraph{Gegeben:}

\[A = \begin{pmatrix}
     2 &  3 & -1\\
    -6 & -5 &  0\\
     2 & -5 &  6
\end{pmatrix},\;\;\; b = \begin{pmatrix}20\\-41\\-15\end{pmatrix}\]

\paragraph{LR-Zerlegung:}

\begin{align}
    &&A^{(0)} &= \begin{gmatrix}[p]
         2 &  3 & -1\\
        -6 & -5 &  0\\
         2 & -5 &  6
        \rowops
        \swap{0}{1}
    \end{gmatrix}\\
    P^{(1)} &= \begin{pmatrix}
        0 & 1 & 0\\
        1 & 0 & 0\\
        0 & 0 & 1
    \end{pmatrix}
    &A^{(1)} &=
    \begin{gmatrix}[p]
        -6 & -5 &  0\\
         2 &  3 & -1\\
         2 & -5 &  6
        \rowops
        \add[\cdot \frac{1}{3}]{0}{1}
        \add[\cdot \frac{1}{3}]{0}{2}
    \end{gmatrix}\\
    L^{(2)} &=\begin{pmatrix}
        1 & 0 & 0\\
      \nicefrac{1}{3} & 1 & 0\\
      \nicefrac{1}{3} & 0 & 1
    \end{pmatrix},
    & A^{(2)} &= \begin{gmatrix}[p]
        -6 & -5 &  0\\
         0 &  \frac{4}{3} & -1\\
         0 & -\frac{20}{3} &  6
        \rowops
        \swap{1}{2}
    \end{gmatrix}\\
    P^{(3)} &= \begin{pmatrix}
        1 & 0 & 0\\
        0 & 0 & 1\\
        0 & 1 & 0
    \end{pmatrix},
    & A^{(3)} &= \begin{gmatrix}[p]
        -6 & -5 &  0\\
         0 & -\frac{20}{3} &  6\\
         0 &  \frac{4}{3} & -1
        \rowops
        \add[\cdot \frac{1}{5}]{1}{2}
    \end{gmatrix}\\
    L^{(4)} &= \begin{pmatrix}
        1 & 0 & 0\\
        0 & 1 & 0\\
        0 & \nicefrac{1}{5} & 1
    \end{pmatrix},
    & A^{(4)} &= \begin{gmatrix}[p]
        -6 & -5 &  0\\
         0 & -\frac{20}{3} &  6\\
         0 &  0 & \nicefrac{1}{5}
    \end{gmatrix} =:R
\end{align}

Es gilt nun:

\begin{align}
    P :&= P^{(3)} \cdot P^{(1)}\\
      &= \begin{pmatrix}
        1 & 0 & 0\\
        0 & 0 & 1\\
        0 & 1 & 0
    \end{pmatrix} \cdot \begin{pmatrix}
        0 & 1 & 0\\
        1 & 0 & 0\\
        0 & 0 & 1
    \end{pmatrix} \\
    &=
    \begin{pmatrix}
        0 & 1 & 0\\
        0 & 0 & 1\\
        1 & 0 & 0
    \end{pmatrix}\\
    L^{(4)} \cdot P^{(3)} \cdot L^{(2)} \cdot P^{(1)} \cdot A &= R\\
L^{-1} &= L^{(4)} \cdot \hat{L_1}\\
    \hat{L_1} &= P^{(3)} \cdot L^{(2)} \cdot (P^{(3)})^{-1}\\
&= P^{(3)} \cdot L^{(2)} \cdot P^{(3)}\\
&= \begin{pmatrix}
        1 & 0 & 0\\
      \nicefrac{1}{3} & 1 & 0\\
      \nicefrac{1}{3} & 0 & 1
    \end{pmatrix}\\
    L &= (L^{(4)} \cdot \hat{L_1})^{-1}\\
    &= \begin{pmatrix}
    1 & 0 & 0\\
    -\frac{1}{3} & 1 & 0\\
    -\frac{1}{3} & -\frac{1}{5} & 1
\end{pmatrix}
\end{align}

Überprüfung mit \href{http://www.wolframalpha.com/input/?i=%7B%7B1%2C+0%2C+0%7D%2C+%7B-1%2F3%2C+1%2C+0%7D%2C+%7B-1%2F3%2C+-1%2F5%2C+1%7D%7D*%7B%7B-6%2C-5%2C0%7D%2C%7B0%2C-20%2F3%2C6%7D%2C%7B0%2C0%2C1%2F5%7D%7D}{Wolfram|Alpha}.
